cleanup pick_left example.

examples/pick_left.v
@@ -16,7 +16,12 @@ Open Scope string_scope.
 
 (* ========================================================================== *)
 
-Example sig := (SigU (SigØ) ("choose") TyUnit (TyΣ TyUnit TyUnit)).
+Definition Bool := (TyΣ TyUnit TyUnit).
+
+Definition TConditional b T1 T2 := TΣMatch b T1 T2.
+
+
+Example sig := (SigU (SigØ) ("choose") TyUnit Bool).
 
 
 Lemma sig_wf:
@@ -29,36 +34,28 @@ Qed.
 Example eq_idem := (EqsU (EqsØ) CtxØ (TCtxU TCtxØ TyUnit)
   (TApp 0 Unit)
   (TOp "choose" Unit 
-    (TΣMatch (Var 0) (TApp 0 Unit) (TApp 0 Unit)))
+    (TConditional (Var 0) (TApp 0 Unit) (TApp 0 Unit)))
 ).
 
 Example eq_idem_assoc := (EqsU eq_idem CtxØ
   (TCtxU (TCtxU (TCtxU TCtxØ TyUnit) TyUnit) TyUnit)
   (TOp "choose" Unit 
-    (TΣMatch (Var 0) 
+    (TConditional (Var 0) 
       (TApp 0 Unit) 
       (TOp "choose" Unit 
-        (TΣMatch (Var 0) (TApp 1 Unit) (TApp 2 Unit)))))
+        (TConditional (Var 0) (TApp 1 Unit) (TApp 2 Unit)))))
   (TOp "choose" Unit 
-    (TΣMatch (Var 0) 
+    (TConditional (Var 0) 
       (TOp "choose" Unit 
-        (TΣMatch (Var 0) (TApp 0 Unit) (TApp 1 Unit)))
+        (TConditional (Var 0) (TApp 0 Unit) (TApp 1 Unit)))
       (TApp 2 Unit) ))
 ).
 
 Lemma eq_idem_wf:
   wf_eqs eq_idem sig.
 Proof.
-assert (forall Γ, wf_ctx Γ -> has_vtype Γ Unit TyUnit).
-{ intros Γ wf. apply TypeV; obvious. apply TypeUnit. }
-unfold eq_idem. apply WfEqsU; obvious.
-- eapply WfTApp; obvious. apply H; obvious. simpl. auto.
-- eapply WfTOp; obvious_vtype.
-  + unfold sig. simpl. reflexivity.
-  + eapply WfTΣMatch.
-    * apply TypeV; obvious. apply TypeVar. simpl. auto.
-    * eapply WfTApp. obvious_vtype. simpl. auto.
-    * eapply WfTApp. obvious_vtype. simpl. auto.
+unfold eq_idem. unfold sig. apply WfEqsU; obvious.
+all: do 4 wft_step; simpl; auto; obvious_vtype.
 Qed.
 
 
@@ -66,22 +63,7 @@ Lemma eq_idem_assoc_wf:
   wf_eqs eq_idem_assoc sig.
 Proof.
 unfold eq_idem_assoc. apply WfEqsU; obvious. apply eq_idem_wf.
-- eapply WfTOp; obvious_vtype.
-  unfold sig. simpl. reflexivity.
-  eapply WfTΣMatch; obvious_vtype.
-  + eapply WfTApp. obvious_vtype. simpl. auto.
-  + eapply WfTOp; obvious_vtype.
-    unfold sig. simpl. reflexivity.
-    eapply WfTΣMatch; obvious_vtype.
-    all: eapply WfTApp; obvious_vtype.
-- eapply WfTOp; obvious_vtype.
-  unfold sig. simpl. reflexivity.
-  eapply WfTΣMatch; obvious_vtype.
-  + eapply WfTOp; obvious_vtype.
-    unfold sig. simpl. reflexivity.
-    eapply WfTΣMatch; obvious_vtype.
-    all: eapply WfTApp; obvious_vtype.
-  + eapply WfTApp. obvious_vtype. simpl. auto.
+all: do 5 (wft_step); simpl; auto; obvious_vtype.
 Qed.
 
 
@@ -101,69 +83,65 @@ Lemma cases_respect D:
 Proof.
 intros wfd.
 unfold sig. unfold eq_idem_assoc.
-apply Respects; obvious. apply eq_idem_assoc_wf.
-apply RespectEqsU. apply Respects; obvious. apply eq_idem_wf.
+apply Respects. 4: apply eq_idem_assoc_wf. all: obvious.
+apply RespectEqsU. apply Respects. 4: apply eq_idem_wf. all: obvious.
 apply RespectEqsU. apply Respects; obvious. apply RespectEqsØ.
 {
-apply ceq_sym. simpl_c_subs.
-assert (has_ctype (CtxU CtxØ (TyFun TyUnit D))
-  (App (Fun (ΣMatch (Var 0) (App (Var 2) Unit) (App (Var 2) Unit))) (Inl Unit))
-  D ).
-{ apply TypeC; obvious. eapply TypeApp. instantiate (1:= TyΣ TyUnit TyUnit).
-  2: obvious_vtype. apply TypeV; obvious. apply TypeFun.
-  apply TypeC; obvious. eapply TypeΣMatch. obvious_vtype.
-  all: obvious_ctype. }
-eapply ceq_trans. apply Ceq. auto. 2: apply βApp.
-{ simpl_c_subs. apply TypeC; obvious. eapply TypeΣMatch. obvious_vtype.
-  all: obvious_ctype. }
-simpl_c_subs. eapply ceq_trans. apply Ceq. 3: apply βΣMatch_Inl.
-{ apply TypeC; obvious. eapply TypeΣMatch. obvious_vtype.
-  all: obvious_ctype. }
-all: simpl_c_subs. obvious_ctype. apply ceq_refl. obvious_ctype.
-}{
-simpl. simpl_c_subs.
+simpl. apply ceq_sym. simpl_c_subs.
 eapply ceq_trans. apply Ceq. 3: apply βApp.
-{ apply TypeC; obvious. eapply TypeApp. instantiate (1:= TyΣ TyUnit TyUnit).
-  + apply TypeV; obvious. apply TypeFun. obvious_ctype. obvious_ctype.
-    apply TypeC; obvious. eapply TypeApp. instantiate (1:= TyΣ TyUnit TyUnit).
-    - apply TypeV; obvious. apply TypeFun.
-      obvious_ctype. all: obvious_ctype.
-    - obvious_vtype.
-  + obvious_vtype. }
-{ simpl_c_subs.
-  apply TypeC; obvious. eapply TypeΣMatch. obvious_vtype. obvious_ctype.
-  apply TypeC; obvious. eapply TypeApp. instantiate (1:= TyΣ TyUnit TyUnit).
-  - apply TypeV; obvious. apply TypeFun.
-    apply TypeC; obvious. eapply TypeΣMatch. obvious_vtype.
-    all: obvious_ctype.
-  - obvious_vtype. }
-simpl_c_subs. apply ceq_sym. eapply ceq_trans. apply Ceq. 3: apply βApp.
-{ ctype_step. instantiate (1:= TyΣ TyUnit TyUnit). vtype_step. obvious_ctype.
-  - ctype_step. instantiate (1:= TyΣ TyUnit TyUnit). vtype_step.
-    obvious_ctype. obvious_ctype. obvious_ctype. obvious_vtype.
-  - obvious_ctype.
-  - obvious_vtype. }
-{ simpl_c_subs. obvious_ctype. 2: obvious_ctype.
-  ctype_step. instantiate (1:= TyΣ TyUnit TyUnit). vtype_step.
-  obvious_ctype; obvious_ctype. obvious_vtype. }
+
+{ ctype_step. instantiate (1:= TyΣ TyUnit TyUnit). 2: obvious_vtype.
+  vtype_step. obvious_ctype; obvious_ctype. }
+{ simpl_c_subs. obvious_ctype; obvious_ctype. }
+
 simpl_c_subs. eapply ceq_trans. apply Ceq. 3: apply βΣMatch_Inl.
-all: simpl_c_subs.
-{ simpl_c_subs. obvious_ctype. 2: obvious_ctype.
-  ctype_step. instantiate (1:= TyΣ TyUnit TyUnit). vtype_step.
-  obvious_ctype; obvious_ctype. obvious_vtype. }
-{ ctype_step. instantiate (1:= TyΣ TyUnit TyUnit). vtype_step.
-  obvious_ctype; obvious_ctype. obvious_vtype. }
-eapply ceq_trans. apply Ceq. 3: apply βApp. all: simpl_c_subs.
-{ ctype_step. instantiate (1:= TyΣ TyUnit TyUnit). vtype_step.
-  obvious_ctype; obvious_ctype. obvious_vtype. }
+
 { obvious_ctype; obvious_ctype. }
+{ simpl_c_subs. obvious_ctype. }
+
+simpl_c_subs. apply ceq_refl. obvious_ctype.
+}
+{
+simpl. simpl_c_subs. eapply ceq_trans. apply Ceq. 3: apply βApp.
+
+{ ctype_step. instantiate (1:= Bool). 2: obvious_vtype.
+  vtype_step. ctype_step. obvious_vtype. obvious_ctype. ctype_step.
+  instantiate (1:= Bool). 2: obvious_vtype. vtype_step. obvious_ctype. }
+{ simpl_c_subs. ctype_step. obvious_vtype. obvious_ctype. ctype_step.
+  instantiate (1:= Bool). 2:obvious_vtype. vtype_step. obvious_ctype. }
+
+simpl_c_subs. apply ceq_sym. eapply ceq_trans. apply Ceq. 3: apply βApp.
+
+{ ctype_step. instantiate (1:= Bool). vtype_step. ctype_step. obvious_vtype.
+  3: obvious_vtype. 2: obvious_ctype. ctype_step. instantiate (1:= Bool).
+  vtype_step. obvious_ctype. obvious_vtype. }
+{ simpl_c_subs. ctype_step. obvious_vtype. 2: obvious_ctype. ctype_step.
+  instantiate (1:= Bool). vtype_step. obvious_ctype. obvious_vtype. }
+
+simpl_c_subs. eapply ceq_trans. apply Ceq. 3: apply βΣMatch_Inl.
+
+{ simpl_c_subs. ctype_step. obvious_vtype. 2: obvious_ctype. ctype_step.
+  instantiate (1:= Bool). vtype_step. obvious_ctype. obvious_vtype. }
+{ simpl_c_subs. ctype_step. instantiate (1:= Bool). vtype_step.
+  obvious_ctype. obvious_vtype. }
+
+simpl_c_subs. eapply ceq_trans. apply Ceq. 3: apply βApp. all: simpl_c_subs.
+
+{ ctype_step. instantiate (1:= Bool). vtype_step.
+  obvious_ctype. obvious_vtype. }
+{ obvious_ctype. }
+
 eapply ceq_trans. apply Ceq. 3: apply βΣMatch_Inl. all: simpl_c_subs.
+
 { obvious_ctype; obvious_ctype. }
 { obvious_ctype. }
+
 eapply ceq_sym. eapply ceq_trans. apply Ceq. 3: apply βΣMatch_Inl.
-{ obvious_ctype. obvious_ctype. ctype_step. instantiate (1:= TyΣ TyUnit TyUnit).
-  vtype_step. obvious_ctype; obvious_ctype. obvious_vtype. }
+
+{ ctype_step. obvious_vtype. obvious_ctype. ctype_step.
+  instantiate (1:= Bool). vtype_step. obvious_ctype. obvious_vtype. }
 { simpl_c_subs. obvious_ctype. }
+
 simpl_c_subs. apply ceq_refl. obvious_ctype.
 }
 Qed.
@@ -175,12 +153,11 @@ Lemma handler_types:
     (TyHandler (CTy TyInt sig eq_idem_assoc) (CTy TyInt SigØ EqsØ))
 .
 specialize eq_idem_assoc_wf as eqwf.
-apply TypeV; obvious.
-apply TypeHandler; obvious.
+vtype_step.
 + obvious_ctype.
 + apply TypeH; obvious. apply TypeCasesU; obvious.
   - apply TypeH; obvious. apply TypeCasesØ.
-  - ctype_step. instantiate (1:= TyΣ TyUnit TyUnit).
+  - ctype_step. instantiate (1:= Bool).
     obvious_vtype. obvious_vtype.
 + apply cases_respect. obvious.
 Qed.
